\documentclass[11pt]{article}
\usepackage{amsmath,amssymb,amsthm}
\linespread{1.8}
\begin{document}
\paragraph{1}
\begin{flalign*}
\begin{split}
<u_N,v> & = \sum_{k=1}^{N}<\mathcal{L}(e_k)e_k,v>\\
& = \sum_{k=1}^{N}\mathcal{L}(e_k)<e_k,v>\\
& = \mathcal{L}(\sum_{k=1}^{N}<e_k,v>e_k)\\
& = \mathcal{L}(v)
\end{split}&
\end{flalign*}
\paragraph{2}
it's obvious that $u_N \in V_N$\\
so $\mathcal{L}(u_N) = \|u_N\|^2$\\
and $\displaystyle \mathcal{L}(u_N) = <\mathcal{L},u_N> \leq \|\mathcal{L}\|\|u_N\|$\\
 $\Rightarrow \|u_N\| \leq \|\mathcal{L}\|$
\paragraph{3}
$\displaystyle \because \|u_N\|^2 = \sum_{k=1}^{N}\mathcal{L}^2(e_k) \leq \|\mathcal{L}\|^2\\
\text{so we have } \sum_{k=1}^{\infty}|\mathcal{L}(e_k)|^2 \leq \|\mathcal{L}\|^2\\
\text{using the lemma in week5 PDF we can know that there exist }u= \sum_{k=1}^{\infty}\mathcal{L}(e_k)e_k\\
\text{which prove the convergence of }\sum_{k=1}^{\infty}\mathcal{L}(e_k)e_k\\
\because u = \sum_{k=1}^{\infty}<u,e_k>e_k\\
\|u - u\| = |\mathcal{L}(e_k) - <u,e_k>|^2 = 0\\
\therefore <u,e_k> = \mathcal{L}(e_k) \; \forall k = 1 \dots \\
\therefore \forall v \in \mathcal{H} v = \sum_{k=1}^{\infty}<v,e_k>e_k\\
\mathcal{L}(v) = \mathcal{L}(\sum_{k=1}^{\infty}<v,e_k>e_k) = \sum_{k=1}^{\infty}<v,e_k>\mathcal{L}(e_k)\\
 = <v,\sum_{k =1}^{\infty}\mathcal{L}(e_k)e_k> = <u,v>\\
 \text{then prove the uniqueness of }u \; \text{if we have a}u^* \;s.t\; \forall v \\
 <u^*,v> = \mathcal{L}(v)\\ 
 \text{then}<u^*,v> = \mathcal{L}(e_k) \; \forall k \geq 0\\
 u^* = \sum_{k=1}^{\infty}<u^*,e_k>e_k = \sum_{k=1}^{\infty}\mathcal{L}(e_k)e_k = u\\
$
\end{document}
